rocq-skylabs-cpp2v/tests/templates/dependent_name_printers.t/test.v
@@ -1,5 +1,8 @@
 Require Import skylabs.prelude.base.
-Require Import skylabs.lang.cpp.mparser.
+Require Import skylabs.lang.cpp.syntax.
+Require Import skylabs.lang.cpp.syntax.templates.
+Require Import skylabs.lang.cpp.mparser (Nlocal).
+
 Require Import test_17_cpp_templates.
 
 Definition lookup_function (n : name) : option Func :=
@@ -12,7 +15,7 @@ Definition lookup_function (n : name) : option Func :=
   | None => None
   end.
 
-Definition lookup_body (n : Mname) : option MStmt :=
+Definition lookup_body (n : name) : option Stmt :=
   match lookup_function n with
   | Some f =>
     match f.(f_body) with
@@ -23,87 +26,87 @@ Definition lookup_body (n : Mname) : option MStmt :=
   end.
 
 Definition template_function_name
-    (name : ident) (params : list Mtype) (args : list Mtemp_arg) : Mname :=
-  Ninst (Nglobal (Nfunction function_qualifiers.N name params)) args.
+    (nm : ident) (params : list type) (args : list temp_arg) : name :=
+  Ninst (Nglobal (Nfunction function_qualifiers.N nm params)) args.
 
-Definition known : Mtype := Tnamed (Nglobal (Nid "Known")).
-Definition known_ptr : Mtype := Tptr known.
+Definition known : type := Tnamed (Nglobal (Nid "Known")).
+Definition known_ptr : type := Tptr known.
 
-Definition paren_member_call_name : Mname :=
+Definition paren_member_call_name : name :=
   template_function_name "paren_member_call" [known_ptr] [Atype (Tparam "T")].
 
-Definition cast_member_call_name : Mname :=
+Definition cast_member_call_name : name :=
   template_function_name "cast_member_call" [known_ptr] [Atype (Tparam "T")].
 
-Definition pseudo_destructor_name : Mname :=
+Definition pseudo_destructor_name : name :=
   template_function_name "pseudo_destructor" [Tptr (Tparam "T")] [Atype (Tparam "T")].
 
-Definition unresolved_member_name : Mname :=
+Definition unresolved_member_name : name :=
   template_function_name "unresolved_member" [Tparam "T"] [Atype (Tparam "T")].
 
-Definition unresolved_conversion_name : Mname :=
+Definition unresolved_conversion_name : name :=
   template_function_name "unresolved_conversion" [Tparam "T"] [Atype (Tparam "T")].
 
-Definition paren_call_name : Mname :=
+Definition paren_call_name : name :=
   template_function_name "paren_call" [Tparam "F"] [Atype (Tparam "F")].
 
-Definition scope_value_name : Mname :=
+Definition scope_value_name : name :=
   template_function_name "scope_value" [] [Atype (Tparam "T")].
 
-Definition scope_call_name : Mname :=
+Definition scope_call_name : name :=
   template_function_name "scope_call" [] [Atype (Tparam "T")].
 
-Definition scope_template_call_name : Mname :=
+Definition scope_template_call_name : name :=
   template_function_name "scope_template_call" [] [Atype (Tparam "T")].
 
-Definition member_value_name : Mname :=
+Definition member_value_name : name :=
   template_function_name "member_value" [Tparam "T"] [Atype (Tparam "T")].
 
-Definition arrow_member_value_name : Mname :=
+Definition arrow_member_value_name : name :=
   template_function_name "arrow_member_value" [Tptr (Tparam "T")] [Atype (Tparam "T")].
 
-Definition member_template_call_name : Mname :=
+Definition member_template_call_name : name :=
   template_function_name "member_template_call" [Tparam "T"] [Atype (Tparam "T")].
 
-Definition adl_call_name : Mname :=
+Definition adl_call_name : name :=
   template_function_name "adl_call" [Tparam "T"] [Atype (Tparam "T")].
 
-Definition unary_plus_name : Mname :=
+Definition unary_plus_name : name :=
   template_function_name "unary_plus" [Tparam "T"] [Atype (Tparam "T")].
 
-Definition binary_plus_name : Mname :=
+Definition binary_plus_name : name :=
   template_function_name "binary_plus" [Tparam "T"; Tparam "T"] [Atype (Tparam "T")].
 
-Definition subscript_name : Mname :=
+Definition subscript_name : name :=
   template_function_name "subscript" [Tparam "T"] [Atype (Tparam "T")].
 
-Definition pointer_to_member_name : Mname :=
+Definition pointer_to_member_name : name :=
   template_function_name "pointer_to_member"
     [Tparam "T"; Tmember_pointer (Tparam "T") Tint] [Atype (Tparam "T")].
 
 Example paren_member_call_body :
   lookup_body paren_member_call_name =
   Some (Sseq [
-    Sreturn_val
-      (Emember_call true
+    Sreturn
+      (Some (Emember_call true
         (inl ((Nscoped (Nglobal (Nid "Known"))
                   (Nfunction function_qualifiers.N "member" [])),
               Direct,
-              Tfunction Mtype CC_C Ar_Definite Tint []))
-        (Ecast Cl2r (Evar "p" known_ptr)) [])
+              "int()"%cpp_type))
+        (Ecast Cl2r (Evar "p" known_ptr)) []))
   ]).
 Proof. vm_compute. reflexivity. Qed.
 
 Example cast_member_call_body :
   lookup_body cast_member_call_name =
   Some (Sseq [
-    Sreturn_val
+    Sreturn (Some
       (Emember_call true
         (inl ((Nscoped (Nglobal (Nid "Known"))
                   (Nop_conv function_qualifiers.N Tint)),
               Direct,
-              Tfunction Mtype CC_C Ar_Definite Tint []))
-        (Ecast Cl2r (Evar "p" known_ptr)) [])
+              "int()"%cpp_type))
+        (Ecast Cl2r (Evar "p" known_ptr)) []))
   ]).
 Proof. vm_compute. reflexivity. Qed.
 
@@ -119,129 +122,129 @@ Proof. vm_compute. reflexivity. Qed.
 Example unresolved_member_body :
   lookup_body unresolved_member_name =
   Some (Sseq [
-    Sreturn_val
+    Sreturn (Some
       (Eunresolved_call
         (Ndependent
-          (Tresult_member (Tparam "T") (Nlocal (Nid "member")))) [])
+          (Tresult_member (Tparam "T") (Nlocal (Nid "member")))) []))
   ]).
 Proof. vm_compute. reflexivity. Qed.
 
 Example unresolved_conversion_body :
   lookup_body unresolved_conversion_name =
   Some (Sseq [
-    Sreturn_val
+    Sreturn (Some
       (Eunresolved_call
         (Ndependent
           (Tresult_member (Tparam "T")
-            (Nlocal (Nop_conv function_qualifiers.N Tint)))) [])
+            (Nlocal (Nop_conv function_qualifiers.N Tint)))) []))
   ]).
 Proof. vm_compute. reflexivity. Qed.
 
 Example paren_call_body :
   lookup_body paren_call_name =
   Some (Sseq [
-    Sreturn_val (Eunresolved_call (Nlocal (Nid "f")) [])
+    Sreturn (Some (Eunresolved_call (Nlocal (Nid "f")) []))
   ]).
 Proof. vm_compute. reflexivity. Qed.
 
 Example scope_value_body :
   lookup_body scope_value_name =
   Some (Sseq [
-    Sreturn_val
-      (Eunresolved_global (Nscoped (Ndependent (Tparam "T")) (Nid "value")))
+    Sreturn (Some
+      (Eunresolved_global (Nscoped (Ndependent (Tparam "T")) (Nid "value"))))
   ]).
 Proof. vm_compute. reflexivity. Qed.
 
 Example scope_call_body :
   lookup_body scope_call_name =
   Some (Sseq [
-    Sreturn_val
+    Sreturn (Some
       (Eunresolved_call
-        (Nscoped (Ndependent (Tparam "T")) (Nid "func")) [])
+        (Nscoped (Ndependent (Tparam "T")) (Nid "func")) []))
   ]).
 Proof. vm_compute. reflexivity. Qed.
 
 Example scope_template_call_body :
   lookup_body scope_template_call_name =
   Some (Sseq [
-    Sreturn_val
+    Sreturn (Some
       (Eunresolved_call
         (Ninst (Nscoped (Ndependent (Tparam "T")) (Nid "func"))
-          [Atype Tint]) [])
+          [Atype Tint]) []))
   ]).
 Proof. vm_compute. reflexivity. Qed.
 
 Example member_value_body :
   lookup_body member_value_name =
   Some (Sseq [
-    Sreturn_val
+    Sreturn (Some
       (core.Eunresolved_member
-        (Evar "p" (Tparam "T")) (Nlocal (Nid "value")))
+        (Evar "p" (Tparam "T")) (Nlocal (Nid "value"))))
   ]).
 Proof. vm_compute. reflexivity. Qed.
 
 Example arrow_member_value_body :
   lookup_body arrow_member_value_name =
   Some (Sseq [
-    Sreturn_val
+    Sreturn (Some
       (core.Eunresolved_member
         (Eunresolved_unop Rarrow
           (Ecast Cl2r (Evar "p" (Tptr (Tparam "T")))))
-        (Nlocal (Nid "value")))
+        (Nlocal (Nid "value"))))
   ]).
 Proof. vm_compute. reflexivity. Qed.
 
 Example member_template_call_body :
   lookup_body member_template_call_name =
   Some (Sseq [
-    Sreturn_val
+    Sreturn (Some
       (Eunresolved_call
         (Ndependent
           (Tresult_member (Tparam "T")
-            (Ninst (Nlocal (Nid "func")) [Atype Tint]))) [])
+            (Ninst (Nlocal (Nid "func")) [Atype Tint]))) []))
   ]).
 Proof. vm_compute. reflexivity. Qed.
 
 Example adl_call_body :
   lookup_body adl_call_name =
   Some (Sseq [
-    Sreturn_val
+    Sreturn (Some
       (Eunresolved_call
-        (Nlocal (Nid "adl_target")) [Evar "p" (Tparam "T")])
+        (Nlocal (Nid "adl_target")) [Evar "p" (Tparam "T")]))
   ]).
 Proof. vm_compute. reflexivity. Qed.
 
 Example unary_plus_body :
   lookup_body unary_plus_name =
   Some (Sseq [
-    Sreturn_val (Eunop Uplus (Evar "p" (Tparam "T")) None)
+    Sreturn (Some (Eunresolved_unop (Runop Uplus) (Evar "p" (Tparam "T"))))
   ]).
 Proof. vm_compute. reflexivity. Qed.
 
 Example binary_plus_body :
   lookup_body binary_plus_name =
   Some (Sseq [
-    Sreturn_val
-      (Ebinop Badd
+    Sreturn (Some
+      (Eunresolved_binop (Rbinop Badd)
         (Evar "a" (Tparam "T"))
-        (Evar "b" (Tparam "T")) None)
+        (Evar "b" (Tparam "T"))))
   ]).
 Proof. vm_compute. reflexivity. Qed.
 
 Example subscript_body :
   lookup_body subscript_name =
   Some (Sseq [
-    Sreturn_val
-      (Esubscript (Evar "p" (Tparam "T")) (Eint 0%Z Tint) None)
+    Sreturn (Some
+      (Eunresolved_binop Rsubscript (Evar "p" (Tparam "T")) (Eint 0%Z Tint)))
   ]).
 Proof. vm_compute. reflexivity. Qed.
 
 Example pointer_to_member_body :
   lookup_body pointer_to_member_name =
   Some (Sseq [
-    Sreturn_val
-      (Ebinop Bdotp
+    Sreturn (Some
+      (Eunresolved_binop (Rbinop Bdotp)
         (Evar "obj" (Tparam "T"))
-        (Evar "member" (Tmember_pointer (Tparam "T") Tint)) None)
+        (Evar "member" (Tmember_pointer (Tparam "T") Tint))))
   ]).
 Proof. vm_compute. reflexivity. Qed.
